src/Language/PlutusIR/Semantics/SemanticEquivalence/Def.v
@@ -10,180 +10,46 @@ Require Import Arith.
 Definition terminates := fun t k => exists v j, j < k /\ t =[j]=> v.
 
 Lemma e : forall i j k,
-  i < k ->
-  j < k - i ->
-  j < k.
+i < k ->
+j < k - i ->
+j < k.
 Proof. Admitted.
-
 
 (* Note: The cases for Ty_Forall and and Ty_IFix make use of
    type substitution and beta reduction. However, Coq can then not
    guess the decreasing argument of fix anymore. *)
 Equations? R (k : nat ) (T : Ty) (t1 t2 : Term) : Prop by wf k :=
   R k T t1 t2 =>
-  emptyContext |-+ t1 : T /\
-  emptyContext |-+ t2 : T /\
-  forall v1 j1,
-    forall (Hj1 : j1 < k),
-    t1 =[j1]=> v1 ->
-    exists v2 j2,
-      t2 =[j2]=> v2 /\
-        match T with
-        | Ty_Forall X K T0 => 
-            forall t0_1 t0_2 T' j,
-              forall (Hj : j < k - j1),
-              v1 = TyAbs X K t0_1 ->
-              v2 = TyAbs X K t0_2 ->
-              emptyContext |-* T' : K ->
-              R j (beta_reduce (substituteT X T' T0)) v1 v2
-        | Ty_Fun T1 T2 => 
-            forall s1 s2 j,
-              forall (Hj : j < k - j1),
-              R j T1 s1 s2 ->
-              R j T2 (Apply v1 s1) (Apply v2 s2)
-        | Ty_Builtin st => 
-            v1 = v2
-        | Ty_IFix F T0 => 
-            forall X K j,
-              forall (Hj : j < k - j1),
-              emptyContext |-* T0 : K ->
-              R j (beta_reduce (unwrapIFix F X K T0)) v1 v2
-        | _ => False (* Ty_Lam, Ty_Abs and Ty_Var should not occur *)
-        end.
+    emptyContext |-+ t1 : T /\
+    emptyContext |-+ t2 : T /\
+    forall v1 j1,
+      forall (Hj1 : j1 < k),
+      t1 =[j1]=> v1 ->
+      exists v2 j2,
+        t2 =[j2]=> v2 /\
+          match T with
+          | Ty_Forall X K T0 => 
+              forall t0_1 t0_2 T' j,
+                forall (Hj : j < k - j1),
+                v1 = TyAbs X K t0_1 ->
+                v2 = TyAbs X K t0_2 ->
+                emptyContext |-* T' : K ->
+                R j (beta_reduce (substituteT X T' T0)) v1 v2
+          | Ty_Fun T1 T2 => 
+              forall s1 s2 j,
+                forall (Hj : j < k - j1),
+                R j T1 s1 s2 ->
+                R j T2 (Apply v1 s1) (Apply v2 s2)
+          | Ty_Builtin st => 
+              v1 = v2
+          | Ty_IFix F T0 => 
+              forall X K j,
+                forall (Hj : j < k - j1),
+                emptyContext |-* T0 : K ->
+                R j (beta_reduce (unwrapIFix F X K T0)) v1 v2
+          | _ => False (* Ty_Lam, Ty_Abs and Ty_Var should not occur *)
+          end.
 Proof. all: try solve [eapply e; eauto]. Qed.
-
-Lemma monotonicity : forall k T v1 v2 j,
-  value v1 ->
-  value v2 ->
-  j <= k ->
-  R k T v1 v2 ->
-  R j T v1 v2.
-Proof.
-  destruct T.
-  - intros.
-    autorewrite with R in H2.
-    autorewrite with R.
-    destruct H2.
-    destruct H3.
-    split; auto.
-    split; auto.
-    intros.
-    assert (j1 < k). {
-      eapply le_trans; eauto.
-    }
-
-    edestruct H4; eauto.
-  - intros.
-    autorewrite with R in H2.
-    autorewrite with R.
-    destruct H2.
-    destruct H3.
-    split; auto.
-    split; auto.
-    intros.
-    assert (j1 < k). {
-      eapply le_trans; eauto.
-    }
-
-    edestruct H4; eauto.
-    destruct H7.
-    destruct H7.
-    exists x.
-    exists x0.
-    split; auto.
-
-    intros.
-    eapply H8.
-    + apply skip. 
-    + assumption.
-  - intros.
-    autorewrite with R in H2.
-    autorewrite with R.
-    destruct H2.
-    destruct H3.
-    split; auto.
-    split; auto.
-    intros.
-    assert (j1 < k). {
-      eapply le_trans; eauto.
-    }
-
-    edestruct H4; eauto.
-    destruct H7.
-    destruct H7.
-    exists x.
-    exists x0.
-    split; auto.
-
-    intros.
-    eapply H8.
-    + apply skip. 
-    + assumption.
-  - intros.
-    autorewrite with R in H2.
-    autorewrite with R.
-    destruct H2.
-    destruct H3.
-    split; auto.
-    split; auto.
-    intros.
-    assert (j1 < k). {
-      eapply le_trans; eauto.
-    }
-
-    edestruct H4; eauto.
-    destruct H7.
-    destruct H7.
-    exists x.
-    exists x0.
-    split; auto.
-
-    intros.
-    eapply H8.
-    + apply skip. 
-    + eassumption.
-    + eassumption.
-    + eassumption.
-  - intros.
-    autorewrite with R in H2.
-    autorewrite with R.
-    destruct H2.
-    destruct H3.
-    split; auto.
-    split; auto.
-    intros.
-    assert (j1 < k). {
-      eapply le_trans; eauto.
-    }
-
-    edestruct H4; eauto.
-  - intros.
-    autorewrite with R in H2.
-    autorewrite with R.
-    destruct H2.
-    destruct H3.
-    split; auto.
-    split; auto.
-    intros.
-    assert (j1 < k). {
-      eapply le_trans; eauto.
-    }
-
-    edestruct H4; eauto.
-  - intros.
-    autorewrite with R in H2.
-    autorewrite with R.
-    destruct H2.
-    destruct H3.
-    split; auto.
-    split; auto.
-    intros.
-    assert (j1 < k). {
-      eapply le_trans; eauto.
-    }
-
-    edestruct H4; eauto.
-Qed.
 
 Lemma R_typable_empty : forall k T t1 t2,
     R k T t1 t2 ->
@@ -281,113 +147,8 @@ Proof.
 Qed.
 
 Lemma R_nontermination : forall k T t1 t2,
-    ~(terminates t1) ->
+    ~(terminates t1 k) ->
     emptyContext |-+ t1 : T ->
     emptyContext |-+ t2 : T ->
     R k T t1 t2.
-Proof. intros. destruct k; destruct T; try solve [split; eauto; split; eauto; intros v1 Hcon; exfalso; apply H; exists v1; auto]. Qed.
-
-(* TODO: Possible fixes for R require a proof of well-founded recursion. I've tried out some things
-   below, but I have not founda solution yet. *)
-(* https://coq.inria.fr/refman/addendum/program.html *)
-(* http://adam.chlipala.net/cpdt/html/Cpdt.GeneralRec.html *)
-
-Fixpoint countBindingLocations (T : Ty) : nat := 
-  match T with
-  | Ty_Var X => 0
-  | Ty_Fun T1 T2 => countBindingLocations T1 + countBindingLocations T2
-  | Ty_IFix F T0 => countBindingLocations F + countBindingLocations T0
-  | Ty_Forall X K T0 => 1 + countBindingLocations T0
-  | Ty_Builtin st => 0
-  | Ty_Lam X K T0 => 1 + countBindingLocations T0       
-  | Ty_App T1 T2 => countBindingLocations T1 + countBindingLocations T2  
-  end.
-
-Program Fixpoint R'' (T : Ty) (t1 t2 : Term) {measure (countBindingLocations T)} : Prop :=
-  emptyContext |-+ t1 : T /\
-  emptyContext |-+ t2 : T /\
-  exists v1 v2,
-    t1 ==> v1 /\
-    t2 ==> v2 /\
-    match T with
-    | Ty_Forall X K T0 => 
-        forall t0 T',
-          v1 = TyAbs X K t0 ->
-          v2 = TyAbs X K t0 ->
-          emptyContext |-* T' : K ->
-          R'' (Named.beta_reduce (substituteT X T' T0)) (TyInst v1 T') (TyInst v2 T')
-    | Ty_Fun T1 T2 => 
-        forall s1 s2,
-          R'' T1 s1 s2 ->
-          R'' T2 (Apply v1 s1) (Apply v2 s2)
-    | Ty_Builtin st => 
-        v1 = v2
-    | Ty_IFix F T0 => 
-        forall X K,
-          emptyContext |-* T : K ->
-          R'' (Named.beta_reduce (unwrapIFix F X K T0)) (Unwrap v1) (Unwrap v2)
-    |_ => False
-    end.
-Next Obligation. Admitted.
-Next Obligation. Admitted.
-Next Obligation. Admitted.
-Next Obligation. Admitted.
-Next Obligation. Admitted.
-Next Obligation. Admitted.
-Next Obligation. Admitted.
-Next Obligation. Admitted.
-
-(* WF by countBindingLocations and size? *)
-Equations R' (T : Ty) (t1 t2 : Term) : Prop by wf (countBindingLocations T) :=
-  R' T t1 t2 =>
-    emptyContext |-+ t1 : T /\
-    emptyContext |-+ t2 : T /\
-    exists v1 v2,
-      t1 ==> v1 /\
-      t2 ==> v2 /\
-      match T with
-      | Ty_Forall X K T0 => 
-          forall t0 T',
-            v1 = TyAbs X K t0 ->
-            v2 = TyAbs X K t0 ->
-            emptyContext |-* T' : K ->
-            R' (Named.beta_reduce (substituteT X T' T0)) (TyInst v1 T') (TyInst v2 T')
-      | Ty_Fun T1 T2 => 
-          forall s1 s2,
-            R' T1 s1 s2 ->
-            R' T2 (Apply v1 s1) (Apply v2 s2)
-      | Ty_Builtin st => 
-          v1 = v2
-      | Ty_IFix F T0 => 
-          forall X K,
-            emptyContext |-* T : K ->
-            R' (Named.beta_reduce (unwrapIFix F X K T0)) (Unwrap v1) (Unwrap v2)
-      |_ => False
-      end.
-      
-
-Fail Inductive R : Ty -> Term -> Term -> Prop :=
-  | R_ : forall t1 t2 T,
-      (emptyContext |-+ t1 : T /\
-      emptyContext |-+ t2 : T /\
-      exists v1 v2,
-        t1 ==> v1 /\
-        t2 ==> v2 /\
-        R2 T v1 v2) ->
-      R T t1 t2
-      
-with R2 : Ty -> Term -> Term -> Prop :=
-  | R2_TyForall : forall X K T0,
-      forall v1 v2 t0 T' S,
-        v1 = TyAbs X K t0 ->
-        v2 = TyAbs X K t0 ->
-        emptyContext |-+ t0 : T0 ->
-        emptyContext |-* T' : K ->
-        substituteT X T' T0 =b S ->
-        R S (TyInst v1 T') (TyInst v2 T') ->
-        R2 (Ty_Forall X K T0) v1 v2
-  | R2_TyFun : forall T1 T2 v1 v2,
-      (forall s1 s2,
-        R T1 s1 s2 ->
-        R T2 (Apply v1 s1) (Apply v2 s2)) ->
-      R2 (Ty_Fun T1 T2) v1 v2.
+Proof. intros. unfold terminates in H. destruct T; try solve [split; auto; split; auto; intros; exfalso; apply H; eauto]. Qed.
