src/Language/PlutusIR/Semantics/SemanticEquivalence/Monotonicity.v
@@ -1,0 +1,147 @@
+Require Import PlutusCert.Language.PlutusIR.
+Import NamedTerm.
+Require Import PlutusCert.Language.PlutusIR.Semantics.Static.
+Require Import PlutusCert.Language.PlutusIR.Semantics.Static.Implementations.Named.
+Require Import PlutusCert.Language.PlutusIR.Semantics.Dynamic.
+Require Import PlutusCert.Language.PlutusIR.Semantics.SemanticEquivalence.Def.
+
+Require Import Arith.
+
+Lemma e2 : forall j j0 k j1,
+    j <= k ->
+    j0 < j - j1 ->
+    j0 < k - j1.
+Proof. Admitted.
+
+Lemma R_monotone : forall k T v1 v2 j,
+  value v1 ->
+  value v2 ->
+  j <= k ->
+  R k T v1 v2 ->
+  R j T v1 v2.
+Proof.
+  destruct T.
+  - intros.
+    autorewrite with R in H2.
+    autorewrite with R.
+    destruct H2.
+    destruct H3.
+    split; auto.
+    split; auto.
+    intros.
+    assert (j1 < k). {
+      eapply le_trans; eauto.
+    }
+
+    edestruct H4; eauto.
+  - intros.
+    autorewrite with R in H2.
+    autorewrite with R.
+    destruct H2.
+    destruct H3.
+    split; auto.
+    split; auto.
+    intros.
+    assert (j1 < k). {
+      eapply le_trans; eauto.
+    }
+
+    edestruct H4; eauto.
+    destruct H7.
+    destruct H7.
+    exists x.
+    exists x0.
+    split; auto.
+
+    intros.
+    eapply H8.
+    + apply e2 with j; auto.
+    + assumption.
+  - intros.
+    autorewrite with R in H2.
+    autorewrite with R.
+    destruct H2.
+    destruct H3.
+    split; auto.
+    split; auto.
+    intros.
+    assert (j1 < k). {
+      eapply le_trans; eauto.
+    }
+
+    edestruct H4; eauto.
+    destruct H7.
+    destruct H7.
+    exists x.
+    exists x0.
+    split; auto.
+
+    intros.
+    eapply H8.
+    + apply e2 with j; auto.
+    + assumption.
+  - intros.
+    autorewrite with R in H2.
+    autorewrite with R.
+    destruct H2.
+    destruct H3.
+    split; auto.
+    split; auto.
+    intros.
+    assert (j1 < k). {
+      eapply le_trans; eauto.
+    }
+
+    edestruct H4; eauto.
+    destruct H7.
+    destruct H7.
+    exists x.
+    exists x0.
+    split; auto.
+
+    intros.
+    eapply H8.
+    + apply e2 with j; auto.
+    + eassumption.
+    + eassumption.
+    + eassumption.
+  - intros.
+    autorewrite with R in H2.
+    autorewrite with R.
+    destruct H2.
+    destruct H3.
+    split; auto.
+    split; auto.
+    intros.
+    assert (j1 < k). {
+      eapply le_trans; eauto.
+    }
+
+    edestruct H4; eauto.
+  - intros.
+    autorewrite with R in H2.
+    autorewrite with R.
+    destruct H2.
+    destruct H3.
+    split; auto.
+    split; auto.
+    intros.
+    assert (j1 < k). {
+      eapply le_trans; eauto.
+    }
+
+    edestruct H4; eauto.
+  - intros.
+    autorewrite with R in H2.
+    autorewrite with R.
+    destruct H2.
+    destruct H3.
+    split; auto.
+    split; auto.
+    intros.
+    assert (j1 < k). {
+      eapply le_trans; eauto.
+    }
+
+    edestruct H4; eauto.
+Qed.
